Minor change

icounter.fst
@@ -3,29 +3,33 @@ module Icounter
 open FStar.List.Tot
 
 type op =
-     | Inc : nat -> op
+  |Inc 
 
-type o = (nat (*unique id*) * op)
+type o = (nat (*unique id*) * op * nat (*element*))
+
+let get_id (id,_,_) = id
+let get_op (_,op,_) = op
+let get_ele (_,_,ele) = ele
 
 type s = nat
-     
+
 val app_op : s -> o -> s
-let app_op c (_,Inc n) = c + n
-  
+let app_op c (_,Inc,n) = c + n
+
 val member : id:nat 
            -> l:list o
-           -> Tot (b:bool{(exists n. mem (id,n) l) <==> b=true})
+           -> Tot (b:bool{(exists op ele. mem (id,op,ele) l) <==> b=true})
 let rec member n l =
   match l with
   |[] -> false
-  |(id,_)::xs -> (n = id) || member n xs
+  |(id,_,_)::xs -> (n = id) || member n xs
 
 val unique : l:list o
            -> Tot bool
 let rec unique l =
   match l with
   |[] -> true
-  |(id,_)::xs -> not (member id xs) && unique xs
+  |(id,_,_)::xs -> not (member id xs) && unique xs
 
 noeq type ae  =
      |A : vis : (o -> o -> Tot bool)
@@ -37,34 +41,39 @@ noeq type ae  =
 
 val sum : a:(list o) -> Tot nat (decreases a)
 let rec sum l =
-  match l with
-  |[] -> 0
-  |((_,Inc n)::xs) -> n + sum xs
-
+     match l with
+     |[] -> 0
+     |((_,Inc, n)::xs) -> n + sum xs
+     
 #set-options "--query_stats"              
 val sim : tr:ae
         -> s1:s 
-        -> Tot bool        
-let sim tr s1 = (s1 = sum tr.l)
+        -> Tot (bool) 
+let rec sim tr s1 = (s1 = sum tr.l)
 
 val rem1 : l:ae 
          -> op:o
          -> Pure (list o)
            (requires true)
-           (ensures (fun r -> (forall n. ((snd op = (Inc n) /\ mem op l.l /\ l.l <> []) ==> (sum r = sum l.l - n))) /\ 
-                           (forall ele. mem ele r ==> mem ele l.l) /\ (unique r))) (decreases %[l.l])
+           (ensures (fun r -> (forall n. ((get_op op = Inc /\ get_ele op = n /\ mem op l.l /\ l.l <> []) ==>
+                           (sum r = sum l.l - n))) /\ 
+                           ((forall e. mem e r ==> mem e l.l) /\ (unique r)))) (decreases %[l.l])
 let rec rem1 l op =
     match l with 
     |(A _ []) -> []
     |(A _ (x::xs)) -> if (x = op) then xs else (x::(rem1 (A l.vis xs) op))
-          
+
 val rem : l:ae 
-        -> op:o 
+        -> op:o
         -> Pure ae
           (requires true)
-          (ensures (fun r -> (forall n. ((snd op = (Inc n) /\ mem op l.l /\ l.l <> []) ==> (sum r.l = sum l.l - n))) /\ 
-                          (forall e. mem e r.l ==> mem e l.l) /\
-                          (forall e e1. mem e r.l /\ mem e1 r.l /\ r.vis e e1 ==> mem e l.l /\ mem e1 l.l /\ l.vis e e1)))
+          (ensures (fun r -> (forall n. ((get_op op = Inc /\ get_ele op = n /\ mem op l.l /\ l.l <> [])
+                                ==> (sum r.l = sum l.l - n))) /\  
+                          ((forall e. mem e r.l ==> mem e l.l) /\
+                          (forall e e1. mem e r.l /\ mem e1 r.l /\ r.vis e e1 ==> mem e l.l /\ mem e1 l.l /\ l.vis e e1) /\
+                          (forall e e1. (mem e r.l /\ mem e1 r.l /\ not (r.vis e e1)) ==> (mem e l.l /\ mem e1 l.l /\ not (l.vis e e1))) /\
+                          (forall e e1. (mem e r.l /\ mem e1 r.l /\ not (r.vis e e1 || r.vis e1 e)) ==> 
+                                   (mem e l.l /\ mem e1 l.l /\ not (l.vis e e1 || l.vis e1 e))))))
 let rem l op =
   let res = (rem1 l op) in
   (A (fun o o1 -> mem o l.l && mem o1 l.l && l.vis o o1) res)
@@ -77,7 +86,7 @@ val diff1 : a:ae
                       (forall e e1. (mem e l.l /\ mem e1 a.l ==> mem e a.l /\ a.vis e e1)))
             (ensures (fun d -> (forall e. mem e d <==> mem e a.l /\ not (mem e l.l)) /\
                             (sum d = sum a.l - sum l.l) /\
-                            (forall e. mem e d ==> not (member (fst e) l.l)))) (decreases %[l.l;a.l])
+                            (forall e. mem e d ==> not (member (get_id e) l.l)))) (decreases %[l.l;a.l])
 let rec diff1 a l = 
     match a,l with
     |_,(A _ []) -> a.l
@@ -90,20 +99,23 @@ val diff : a:ae
                     (forall e e1. mem e l.l /\ mem e1 l.l /\ l.vis e e1 ==> mem e a.l /\ mem e1 a.l /\ a.vis e e1) /\
                     (forall e e1. (mem e l.l /\ mem e1 a.l ==> mem e a.l /\ a.vis e e1)))
           (ensures (fun d -> (forall e. mem e d.l <==> mem e a.l /\ not(mem e l.l)) /\
+                          (forall e. mem e d.l ==> not (member (get_id e) l.l)) /\
                           (sum d.l = sum a.l - sum l.l) /\
-                          (forall e. mem e d.l ==> not (member (fst e) l.l)) /\
-                          (forall e e1. mem e d.l /\ mem e1 d.l /\ d.vis e e1 ==> mem e a.l /\ mem e1 a.l /\ a.vis e e1))) (decreases l)
+                          (forall e e1. mem e d.l /\ mem e1 d.l /\ d.vis e e1 ==> mem e a.l /\ mem e1 a.l /\ a.vis e e1) /\
+                          (forall e e1. (mem e d.l /\ mem e1 d.l /\ not (d.vis e e1)) ==> (mem e a.l /\ mem e1 a.l /\ not (a.vis e e1))) /\
+                          (forall e e1. (mem e d.l /\ mem e1 d.l /\ not (d.vis e e1 || d.vis e1 e)) ==>
+                                   (mem e a.l /\ mem e1 a.l /\ not (a.vis e e1 || a.vis e1 e))))) (decreases l)
 let diff a l =
   (A (fun o o1 -> mem o a.l && mem o1 a.l && a.vis o o1) (diff1 a l))
 
 val union1 : a:ae 
            -> b:ae
            -> Pure (list o)
-             (requires (forall e. (mem e a.l ==> not (member (fst e) b.l))) /\
-                             (forall e. (mem e b.l ==> not (member (fst e) a.l))))
-             (ensures (fun u -> (sum u = sum a.l + sum b.l) /\ 
+             (requires (forall e. (mem e a.l ==> not (member (get_id e) b.l))) /\
+                             (forall e. (mem e b.l ==> not (member (get_id e) a.l))))
+             (ensures (fun u -> (sum u = sum a.l + sum b.l) /\  
                              (forall e. mem e u <==> mem e a.l \/ mem e b.l) /\
-                             (unique u)))     (decreases %[a.l;b.l])        
+                             (unique u)))     (decreases %[a.l;b.l])
 let rec union1 a b =
   match a,b with
   |(A _ []),(A _ []) -> []
@@ -113,15 +125,22 @@ let rec union1 a b =
 val union : a:ae 
           -> b:ae
           -> Pure ae
-            (requires (forall e. (mem e a.l ==> not (member (fst e) b.l))) /\
-                            (forall e. (mem e b.l ==> not (member (fst e) a.l))))
-            (ensures (fun u -> (sum u.l = sum a.l + sum b.l) /\ 
+            (requires (forall e. (mem e a.l ==> not (member (get_id e) b.l))) /\
+                            (forall e. (mem e b.l ==> not (member (get_id e) a.l))))
+            (ensures (fun u -> 
                             (forall e. mem e u.l <==> mem e a.l \/ mem e b.l) /\
+                            (sum u.l = sum a.l + sum b.l) /\  
                             (forall e e1. (mem e u.l /\ mem e1 u.l /\ u.vis e e1) <==> 
-                                     ((mem e a.l /\ mem e1 a.l /\ a.vis e e1) \/ (mem e b.l /\ mem e1 b.l /\ b.vis e e1)))))
+                                     ((mem e a.l /\ mem e1 a.l /\ a.vis e e1) \/ (mem e b.l /\ mem e1 b.l /\ b.vis e e1))) /\
+                            (forall e e1. mem e a.l /\ mem e1 a.l /\ not (a.vis e e1) ==> mem e u.l /\ mem e1 u.l /\ not (u.vis e e1)) /\
+                            (forall e e1. mem e b.l /\ mem e1 b.l /\ not (b.vis e e1) ==> mem e u.l /\ mem e1 u.l /\ not (u.vis e e1)) /\
+                            (forall e e1. mem e a.l /\ mem e1 a.l /\ not (a.vis e e1 || a.vis e1 e) ==> 
+                                     mem e u.l /\ mem e1 u.l /\ not (u.vis e e1 || u.vis e1 e)) /\
+                            (forall e e1. mem e b.l /\ mem e1 b.l /\ not (b.vis e e1 || b.vis e1 e) ==> 
+                                     mem e u.l /\ mem e1 u.l /\ not (u.vis e e1 || u.vis e1 e))))
 let union a b = 
   (A (fun o o1 -> (mem o a.l && mem o1 a.l && a.vis o o1) || (mem o b.l && mem o1 b.l && b.vis o o1)) (union1 a b))
-  
+
 val absmerge : l:ae
              -> a:ae
              -> b:ae
@@ -131,13 +150,22 @@ val absmerge : l:ae
                                    mem e1 a.l /\ mem e2 a.l /\ a.vis e1 e2 /\ mem e1 b.l /\ mem e2 b.l /\ b.vis e1 e2) /\
                          (forall e e1. mem e l.l /\ mem e1 a.l ==> a.vis e e1) /\
                          (forall e e1. mem e l.l /\ mem e1 b.l ==> b.vis e e1) /\
-                         (forall e. mem e (diff a l).l ==> not (member (fst e) b.l)) /\
-                         (forall e1. mem e1 (diff b l).l ==> not (member (fst e1) a.l)))  
-                (ensures (fun u -> (forall e. mem e u.l <==> mem e l.l \/ mem e a.l \/ mem e b.l) /\ 
+                         (forall e. mem e (diff a l).l ==> not (member (get_id e) b.l)) /\
+                         (forall e1. mem e1 (diff b l).l ==> not (member (get_id e1) a.l)))  
+                (ensures (fun u ->(forall e. mem e u.l <==> mem e l.l \/ mem e a.l \/ mem e b.l) /\ 
                                (forall e1 e2. (mem e1 u.l /\ mem e2 u.l /\ u.vis e1 e2) <==> 
                                          (mem e1 l.l /\ mem e2 l.l /\ l.vis e1 e2) \/
                                          (mem e1 a.l /\ mem e2 a.l /\ a.vis e1 e2) \/ 
-                                         (mem e1 b.l /\ mem e2 b.l /\ b.vis e1 e2))))
+                                         (mem e1 b.l /\ mem e2 b.l /\ b.vis e1 e2)) /\ 
+                              (forall e e1. mem e l.l /\ mem e1 l.l /\ not (l.vis e e1) ==> mem e u.l /\ mem e1 u.l /\ not (u.vis e e1)) /\
+                              (forall e e1. mem e a.l /\ mem e1 a.l /\ not (a.vis e e1) ==> mem e u.l /\ mem e1 u.l /\ not (u.vis e e1)) /\
+                              (forall e e1. mem e b.l /\ mem e1 b.l /\ not (b.vis e e1) ==> mem e u.l /\ mem e1 u.l /\ not (u.vis e e1)) /\
+                              (forall e e1. mem e l.l /\ mem e1 l.l /\ not (l.vis e e1 || l.vis e1 e) ==> 
+                                       mem e u.l /\ mem e1 u.l /\ not (u.vis e e1 || u.vis e1 e)) /\
+                              (forall e e1. mem e a.l /\ mem e1 a.l /\ not (a.vis e e1 || a.vis e1 e) ==>
+                                       mem e u.l /\ mem e1 u.l /\ not (u.vis e e1 || u.vis e1 e)) /\
+                              (forall e e1. mem e b.l /\ mem e1 b.l /\ not (b.vis e e1 || b.vis e1 e) ==> 
+                                       mem e u.l /\ mem e1 u.l /\ not (u.vis e e1 || u.vis e1 e))))
                                        
 let absmerge l a b = 
     let la = diff a l in
@@ -157,10 +185,10 @@ val lemma : ltr:ae
                            (forall e e1. mem e ltr.l /\ mem e1 atr.l  ==> mem e atr.l /\ atr.vis e e1)) ==> a >= l)
                            (decreases %[ltr.l;atr.l])
 let rec lemma ltr l atr a = 
-  match ltr,atr with
-  |(A _ []), (A _ []) -> ()
-  |(A _ (x::xs)), _ -> lemma (A ltr.vis xs) l atr a
-  |(A _ []), (A _ (x::xs)) -> lemma ltr l (A atr.vis xs) a
+    match ltr,atr with
+    |(A _ []), (A _ []) -> ()
+    |(A _ (x::xs)), _ -> lemma (A ltr.vis xs) l atr a
+    |(A _ []), (A _ (x::xs)) -> lemma ltr l (A atr.vis xs) a
 
 val merge : ltr:ae
           -> l:s
@@ -175,19 +203,20 @@ val merge : ltr:ae
                              (forall e1 e2. (mem e1 ltr.l /\ mem e2 ltr.l /\ ltr.vis e1 e2) <==> 
                                        (mem e1 atr.l /\ mem e2 atr.l /\ atr.vis e1 e2 /\ 
                                         mem e1 btr.l /\ mem e2 btr.l /\ btr.vis e1 e2)) /\
-                             (forall e e1. mem e (diff atr ltr).l /\ mem e1 (diff btr ltr).l ==> 
-                                      not (member (fst e) btr.l) /\ not (member (fst e1) atr.l)))                
-                   (ensures (fun res -> true))                  
+                             (forall e. mem e (diff atr ltr).l  ==> not (member (get_id e) btr.l)) /\
+                             (forall e. mem e (diff btr ltr).l ==> not (member (get_id e) atr.l)))
+                   (ensures (fun res -> true))                         
+
 let merge ltr l atr a btr b = 
-    lemma ltr l atr a;
-    lemma ltr l btr b;
-    a + b - l
+      lemma ltr l atr a;
+      lemma ltr l btr b;
+      a + b - l
 
 val append : tr:ae
            -> op:o
            -> Pure ae
-             (requires (not (member (fst op) tr.l)))
-             (ensures (fun res -> true)) (decreases tr.l)               
+             (requires (not (member (get_id op) tr.l)))
+             (ensures (fun res -> true)) (decreases tr.l)
 let append tr op =
     match tr with
     |(A _ []) -> (A (fun o o1 -> mem o tr.l && mem o1 tr.l && tr.vis o o1) (op::[]))
@@ -202,29 +231,34 @@ val prop_merge : ltr: ae
                -> Lemma (requires (sim ltr l /\ sim atr a /\ sim btr b) /\ 
                                  (forall e. mem e ltr.l <==> mem e atr.l /\ mem e btr.l) /\
                                  (forall e e1. mem e ltr.l /\ mem e1 atr.l ==> mem e atr.l /\ atr.vis e e1) /\
-                                 (forall e e1. mem e ltr.l /\ mem e1 btr.l ==> mem e btr.l /\ btr.vis e e1) /\
+                                 (forall e e1. mem e ltr.l /\ mem e1 btr.l ==>  mem e btr.l /\ btr.vis e e1) /\
                                  (forall e1 e2. (mem e1 ltr.l /\ mem e2 ltr.l /\ ltr.vis e1 e2) <==> 
                                            (mem e1 atr.l /\ mem e2 atr.l /\ atr.vis e1 e2 /\ 
                                            mem e1 btr.l /\ mem e2 btr.l /\ btr.vis e1 e2)) /\
-                                 (forall e e1. mem e (diff atr ltr).l /\ mem e1 (diff btr ltr).l ==> 
-                                          not (member (fst e) btr.l) /\ not (member (fst e1) atr.l)))                        
+                                 (forall e. mem e (diff atr ltr).l  ==> not (member (get_id e) btr.l)) /\
+                                 (forall e. mem e (diff btr ltr).l ==> not (member (get_id e) atr.l)))                        
                        (ensures (sim (absmerge ltr atr btr) (merge ltr l atr a btr b))) 
 
-#set-options "--z3rlimit 30"    
+#set-options "--z3rlimit 30"
 let prop_merge ltr l atr a btr b = ()
-
+ 
 val prop_oper : tr:ae
               -> st:s
               -> op:o 
               -> Lemma (requires (sim tr st) /\ 
-                                (not (member (fst op) tr.l)) /\ 
+                                (not (member (get_id op) tr.l)) /\
                                 (forall e. mem e tr.l ==> (append tr op).vis e op))
                       (ensures (sim (append tr op) (app_op st op))) (decreases %[tr.l])
 let prop_oper tr st op = ()
-          
+
 val convergence : tr:ae
-                -> a:s 
-                -> b:s 
-                -> Lemma (ensures (sim tr a /\ sim tr b) ==> a = b)                      
+                -> a:s
+                -> b:s  
+                -> Lemma (requires (sim tr a /\ sim tr b))
+                        (ensures (a = b))
 let convergence tr a b = ()
 
+
+(* Statistics: 
+
+*)
